Final commit

code/Krivine.ml
@@ -8,22 +8,20 @@ type state = {mutable c:code;mutable e:environment;mutable s:stack};;
 
 let L (S a)=a;;
 
-(*
+
 let rec execute st =
-if st.c=[] then st else
+if (st.c=[]) then st else
 match hd(st.c) with
-|Access 0->execute {c=fst(hd(st.e));e=snd(hd(st.e));s=st.s};
-|Access n->st.c=Access (n-1)::tl(st.c);st.e=tl(st.e);execute st;
-|Grab->st.c=tl(st.c);st.e=hd(st.s)::st.e;st.s=tl(st.s);execute st;
-|Push cc->st.s=(cc,st.e)::st.s;st.c=tl(st.c);execute st;;
-*)
+|Access 0->st.c<-fst(hd(L st.e));st.e<-snd(hd(L st.e));execute st;
+|Access n->st.c<-Access (n-1)::tl(st.c);st.e<-S (tl(L st.e));execute st;
+|Grab->st.c<-tl(st.c);st.e<-S (hd(L st.s)::(L st.e));st.s<-S (tl(L st.s));execute st;
+|Push cc->st.s<-S ((cc,st.e)::(L st.s));st.c<-tl(st.c);execute st;;
 
-let rec execute st =
-if (st.(c)=[]) then st else
-match hd(st.(c)) with
-|Access 0->st.(c)<-fst(hd(L st.(e)));st.(e)<-S snd(hd(L st.(e)));execute st;
-|Access n->st.(c)<-Access (n-1)::tl(st.(c));st.(e)<-S tl(L st.(e));execute st;
-|Grab->st.(c)<-tl(st.(c));st.(e)<-S hd(L st.(s))::(L st.(e));st.(s)<-S tl(L st.(s));execute st;
-|Push cc->st.(s)<-S (cc,L st.(e))::(L st.(s));st.(c)<-tl(st.(c));execute st;;
+type DBT = Var of int | Fun of DBT | Appl of DBT*DBT;;
 
-let st={c:[];e:S [];s:S []};;
+let rec code_of_DBT dbt =
+match dbt with
+|Var n->[Access n]
+|Fun dbt1->Grab::(code_of_DBT dbt1)
+|Appl (dbt1,dbt2)->(Push (code_of_DBT dbt1))::(code_of_DBT dbt2);;
+
